Definition and correctness of Nth

TM/Code/ListTM.v
@@ -5,6 +5,9 @@ Require Import ChangeAlphabet.
 Require Import TM.Compound.TMTac.
 
 
+Local Arguments skipn { A } !n !l.
+
+
 (** * Implementation of [nth_error] *)
 
 Section Nth.
@@ -43,47 +46,47 @@ Section Nth.
    *   }
    * }
    *
-   * t0: n (copy)
-   * t1: l (copy)
+   * t0: l (copy)
+   * t1: n (copy)
    * t2: x (output)
    *)
 
   Definition Nth_Step_Rel : Rel (tapes tau^+ 3) ((bool*unit) * tapes tau^+ 3) :=
     fun tin '(yout, tout) =>
-      forall (n : nat) (l : list X),
-        tin[@Fin0] ≃ n ->
-        tin[@Fin1] ≃ l ->
+      forall (l : list X) (n : nat),
+        tin[@Fin0] ≃ l ->
+        tin[@Fin1] ≃ n ->
         isRight tin[@Fin2] ->
         match n, l with
         | S n', x :: l' => (* Recursion case *)
-          tout[@Fin0] ≃ n' /\
-          tout[@Fin1] ≃ l' /\
+          tout[@Fin0] ≃ l' /\
+          tout[@Fin1] ≃ n' /\
           isRight tout[@Fin2] /\
           yout = (true, tt) (* continue *)
         | S n', nil => (* list to short *)
-          tout[@Fin0] ≃ n' /\
-          tout[@Fin1] ≃ l /\
+          tout[@Fin0] ≃ l /\
+          tout[@Fin1] ≃ n' /\
           tout[@Fin2] ≃ None /\
           yout = (false, tt) (* return None *)
         | 0, x::l' => (* return value *)
-          tout[@Fin0] ≃ 0 /\
-          tout[@Fin1] ≃ l' /\
+          tout[@Fin0] ≃ l' /\
+          tout[@Fin1] ≃ 0 /\
           tout[@Fin2] ≃ Some x /\
           yout = (false, tt) (* return Some x *)
         | 0, nil => (* list to short *)
-          tout[@Fin0] ≃ n /\
-          tout[@Fin1] ≃ l /\
+          tout[@Fin0] ≃ l /\
+          tout[@Fin1] ≃ n /\
           tout[@Fin2] ≃ None /\
           yout = (false, tt) (* return None *)
         end.
 
 
   Definition Nth_Step : { M : mTM tau^+ 3 & states M -> bool*unit } :=
-    If (Inject (ChangeAlphabet MatchNat _) [|Fin0|])
-       (If (Inject (MatchList sigX) [|Fin1; Fin2|])
+    If (Inject (ChangeAlphabet MatchNat _) [|Fin1|])
+       (If (Inject (MatchList sigX) [|Fin0; Fin2|])
            (Return (Inject (Reset _) [|Fin2|]) (true, tt))
            (Return (Inject (Constr_None _) [|Fin2|]) (false, tt)))
-       (If (Inject (MatchList sigX) [|Fin1; Fin2|])
+       (If (Inject (MatchList sigX) [|Fin0; Fin2|])
            (Return (Inject (Constr_Some _) [|Fin2|]) (false, tt))
            (Return (Inject (Constr_None _) [|Fin2|]) (false, tt)))
   .
@@ -103,7 +106,7 @@ Section Nth.
     }
     {
       intros tin ((yout, ()), tout) H.
-      intros n l HEncN HEncL HRight.
+      intros l n HEncL HEncN HRight.
       subst tau. destruct H; TMSimp.
       { (* First "Then" case *)
         specialize (H n). spec_assert H by now eapply contains_translate_tau1.
@@ -120,8 +123,8 @@ Section Nth.
           destruct l as [ | x l']; destruct H0 as (H0&H0'&H0''); inv H0''.
           (* We know that l = x :: l' *)
           repeat split; eauto.
-          - now eapply contains_translate_tau2 in H.
           - eapply tape_contains_ext with (1 := H0). cbn. now rewrite map_id.
+          - now eapply contains_translate_tau2 in H.
         }
         { (* Second "Else" case *)
           specialize (H0 l). spec_assert H0.
@@ -151,8 +154,8 @@ Section Nth.
           destruct l as [ | x l']; destruct H0 as (H0&H0'&H0''); inv H0''.
           (* We know that l = x :: l' *)
           repeat split; eauto.
-          - now eapply contains_translate_tau2 in H.
           - eapply tape_contains_ext with (1 := H0). cbn. now rewrite map_id.
+          - now eapply contains_translate_tau2 in H.
         }
         { (* Second "Else" case *)
           specialize (H0 l). spec_assert H0.
@@ -170,5 +173,69 @@ Section Nth.
   Qed.
 
 
+  Definition Nth_Loop_Rel : Rel (tapes tau^+ 3) (unit * tapes tau^+ 3) :=
+    ignoreParam
+      (fun tin tout =>
+         forall l (n : nat),
+           tin[@Fin0] ≃ l ->
+           tin[@Fin1] ≃ n ->
+           isRight tin[@Fin2] ->
+           tout[@Fin0] ≃ skipn (S n) l /\
+           tout[@Fin1] ≃ n - (S (length l)) /\
+           tout[@Fin2] ≃ nth_error l n).
 
+
+  Definition Nth_Loop := WHILE Nth_Step.
+
+
+  Lemma Nth_Loop_WRealise : Nth_Loop ⊫ Nth_Loop_Rel.
+  Proof.
+    eapply WRealise_monotone.
+    { unfold Nth_Loop. repeat TM_Correct. eapply Nth_Step_WRealise. }
+    {
+      apply WhileInduction; intros; intros l n HEncL HEncN HRight.
+      - TMSimp. specialize (HLastStep _ _ HEncL HEncN HRight).
+        destruct n as [ | n'], l as [ | x l']; destruct HLastStep as (H1&H2&H3&H4); inv H4; cbn; repeat split; eauto.
+        now rewrite Nat.sub_0_r.
+      - TMSimp. specialize (HStar _ _ HEncL HEncN HRight).
+        destruct n as [ | n'], l as [ | x l']; destruct HStar as (H1&H2&H3&H4); inv H4; cbn in *;
+          specialize (HLastStep _ _ H1 H2 H3) as (H4&H5&H6); auto.
+    }
+  Qed.
+
+
+  Definition Nth : { M : mTM tau^+ 5 & states M -> unit } :=
+    Inject (CopyValue _) [|Fin0; Fin3|];; (* Save l (on t0) to t3 and n (on t1) to t4 *)
+    Inject (CopyValue _) [|Fin1; Fin4|];;
+    Inject (Nth_Loop) [|Fin3; Fin4; Fin2|];; (* Execute the loop with the copy of n and l *)
+    Inject (Reset _) [|Fin3|];; (* Reset the copies *)
+    Inject (Reset _) [|Fin4|]
+  .
+
+
+  Lemma Nth_Computes : Nth ⊫ Computes2_Rel (@nth_error _).
+  Proof.
+    eapply WRealise_monotone.
+    { unfold Nth. repeat TM_Correct.
+      - apply CopyValue_WRealise with (X := list X).
+      - apply CopyValue_WRealise with (X := nat).
+      - apply Nth_Loop_WRealise.
+      - apply Reset_WRealise with (X := list X).
+      - apply Reset_WRealise with (X := nat).
+    }
+    {
+      intros tin ((), tout) H. cbn. intros l n HEncL HEncN HOut HInt.
+      specialize (HInt Fin0) as HInt1. specialize (HInt Fin1) as HInt2. clear HInt.
+      TMSimp. (* This can take a while *)
+      specialize H with (1 := HEncL) (2 := HInt1) as (H&H').
+      specialize H0 with (1 := HEncN) (2 := HInt2) as (H0&H0').
+      specialize H1 with (1 := H') (2 := H0') (3 := HOut) as (H1&H1'&H1'').
+      specialize H2 with (1 := H1).
+      specialize H3 with (1 := H1').
+      repeat split; eauto.
+      - intros i. destruct_fin i; TMSimp; auto.
+    }
+  Qed.
+      
+  
 End Nth.
